dev/lf/paths/tight/General_to_tight.v
@@ -8,99 +8,36 @@ Require Import Inert_types.
 Require Import Some_lemmas.
 Require Import Tight_possible_types.
 
-(* ###################################################################### *)
-(** ** Tight to precise *)
-
-(* Lemma 1 *)
-Lemma tight_to_precise_typ_dec: forall G x A S U,
-  inert G ->
-  G |-# trm_path (p_var (avar_f x)) :: typ_rcd (dec_typ A S U) ->
-  exists T,
-    G |-! trm_path (p_var (avar_f x)) :: typ_rcd (dec_typ A T T) /\
-    G |-# T <: U /\
-    G |-# S <: T.
-Proof.
-  introv HG Ht.
-  lets Htp: (tight_possible_types_lemma HG Ht). clear Ht.
-  dependent induction Htp.
-  - lets Hp: (inert_precise_dec_typ_inv HG H). subst.
-    exists U. split*.
-  - specialize (IHHtp A T U0 HG eq_refl).
-    destruct IHHtp as [V [Hx [Hs1 Hs2]]].
-    exists V. split*.
-Qed.
-
-Lemma tight_to_precise_trm_dec: forall G x a m T,
-  inert G ->
-  G |-# trm_path (p_var (avar_f x)) :: typ_rcd {{ a [m] T }} ->
-  exists T',
-    G |-! trm_path (p_var (avar_f x)) :: typ_rcd {{ a [m] T' }} /\
-    G |-# T' <: T.
-Proof.
-  introv Hgd Ht.
-  lets Htp: (tight_possible_types_lemma Hgd Ht). clear Ht.
-  dependent induction Htp.
-  - exists T. auto.
-  - specialize (IHHtp _ _ Hgd eq_refl). destruct IHHtp as [V [Hx Hs]].
-    exists V. split; auto.
-    eapply subtyp_trans; eassumption.
-Qed.
-
-Lemma tight_to_precise_typ_all: forall G x S T,
-  inert G ->
-  G |-# trm_path (p_var (avar_f x)) :: typ_all S T ->
-  exists S' T' L,
-    G |-! trm_path (p_var (avar_f x)) :: typ_all S' T' /\
-    G |-# S <: S' /\
-    (forall y,
-        y \notin L ->
-            G & y ~ S |- T' ||^ y <: T ||^ y).
-Proof.
-  introv HG Ht.
-  lets Htp: (tight_possible_types_lemma HG Ht). clear Ht.
-  dependent induction Htp.
-  - exists S T (dom G); auto.
-  - specialize (IHHtp _ _ HG eq_refl).
-    destruct IHHtp as [S' [T' [L' [Hpt [HSsub HTsub]]]]].
-    exists S' T' (dom G \u L \u L').
-    split; auto.
-    assert (Hsub2 : G |-# typ_all S0 T0 <: typ_all S T).
-    { apply subtyp_all with (L:=L); assumption. }
-    split.
-    + eapply subtyp_trans; eauto.
-    + intros y Fr.
-      assert (Hok: ok (G & y ~ S)) by auto using ok_push, inert_ok.
-      apply tight_to_general in H; auto.
-      assert (Hnarrow: G & y ~ S |- T' ||^ y <: T0 ||^ y).
-      { eapply narrow_subtyping; auto using subenv_last. }
-      eauto.
-Qed.
-
 (* Lemma 2 *)
-Lemma tight_subtyping_sel: forall G x A S U,
+Lemma tight_subtyping_sel: forall G p A S U,
     inert G ->
-    G |-# trm_path (p_var (avar_f x)) :: typ_rcd (dec_typ A S U) ->
-    G |-# typ_path (p_var (avar_f x)) A <: U /\
-    G |-# S <: typ_path (p_var (avar_f x)) A.
+    norm_t G p ->
+    G |-# trm_path p : typ_rcd (dec_typ A S U) ->
+    G |-# typ_path p A <: U /\
+    G |-# S <: typ_path p A.
 Proof.
-  introv HG Hty.
-  pose proof (tight_to_precise_typ_dec HG Hty) as [T [Ht [Hs1 Hs2]]].
+  introv Hi Hn Hty.
+  lets Hp: (tight_possible_types_lemma Hi Hty Hn).
+  pose proof (tpt_to_precise_typ_dec Hi Hn Hp) as [T [Ht [Hs1 Hs2]]].
   split.
-  - apply subtyp_sel1_t in Ht. apply subtyp_trans_t with (T:=T); auto.
-  - apply subtyp_sel2_t in Ht. apply subtyp_trans with (T:=T); auto.
+  - apply subtyp_sel1_t in Ht. apply subtyp_trans_t with (T:=T); auto. assumption.
+  - apply subtyp_sel2_t in Ht. apply subtyp_trans_t with (T:=T); auto. assumption.
 Qed.
 
 (* Theorem 1 *)
-Lemma general_to_tight: forall G0,
-  inert G0 ->
+Lemma general_to_tight: forall G0, inert G0 ->
   (forall G t T,
-     G |- t :: T ->
+     G |- t : T ->
      G = G0 ->
-     G |-# t :: T) /\
+     G |-# t : T) /\
   (forall G S U,
      G |- S <: U ->
      G = G0 ->
-     G |-# S <: U).
+     G |-# S <: U) /\
+  (forall G p,
+      norm G p ->
+      G = G0 ->
+      norm_t G p).
 Proof.
   intros G0 HG.
   apply ts_mutind; intros; subst; try solve [eapply tight_subtyping_sel; auto]; eauto.
@@ -108,8 +45,8 @@ Qed.
 
 Lemma general_to_tight_typing: forall G t T,
   inert G ->
-  G |- t :: T ->
-  G |-# t :: T.
+  G |- t : T ->
+  G |-# t : T.
 Proof.
   intros. apply* general_to_tight.
 Qed.
