dev/lf/paths/tight/Tight_possible_types.v
@@ -5,6 +5,7 @@ Require Import Coq.Program.Equality.
 Require Import Definitions.
 Require Import Inert_types.
 Require Import Some_lemmas.
+Require Import Narrowing.
 
 (* ###################################################################### *)
 (** ** Tight Possible types *)
@@ -24,63 +25,134 @@ If S1 in SS and S2 in SS then (S1 & S2) in SS.
 If S in SS and G |-! y: {A: S..S} then y.A in SS.
  *)
 
-Reserved Notation "G '|-##' p '::' T" (at level 40, p at level 59).
+Reserved Notation "G '|-##' p ':' T" (at level 40, p at level 59).
 
 Inductive tight_pt : ctx -> path -> typ -> Prop :=
   (* Precise typing *)
 | t_pt_precise : forall G p T,
-    G |-! trm_path p :: T ->
-    G |-## p :: T
+    G |-! trm_path p : T ->
+    G |-## p : T
   (* General term member subtyping *)
 | t_pt_dec_trm : forall G p a T T',
-    G |-## p :: typ_rcd {{ a [gen] T }} ->
+    G |-## p : typ_rcd {{ a [gen] T }} ->
     G |-# T <: T' ->
-    G |-## p :: typ_rcd {{ a [gen] T' }}
+    G |-## p : typ_rcd {{ a [gen] T' }}
   (* Strong term member subtyping *)
 | t_pt_dec_trm_strong : forall G p a T,
-    G |-## p :: typ_rcd {{ a [strong] T }} ->
-    G |-## p :: typ_rcd {{ a [gen] T }}
+    G |-## p : typ_rcd {{ a [strong] T }} ->
+    G |-## p : typ_rcd {{ a [gen] T }}
   (* Type member subtyping *)
 | t_pt_dec_typ : forall G p A T T' U' U,
-    G |-## p :: typ_rcd (dec_typ A T U) ->
+    G |-## p : typ_rcd (dec_typ A T U) ->
     G |-# T' <: T ->
     G |-# U <: U' ->
-    G |-## p :: typ_rcd (dec_typ A T' U')
+    G |-## p : typ_rcd (dec_typ A T' U')
   (* Recursive Types *)
 | t_pt_bnd : forall G x S,
-    G |-## (p_var (avar_f x)) :: S ||^ x ->
-    G |-## (p_var (avar_f x)) :: typ_bnd S
+    G |-## (p_var (avar_f x)) : S ||^ x ->
+    G |-## (p_var (avar_f x)) : typ_bnd S
   (* Forall *)
 | t_pt_all : forall L G p S T S' T',
-    G |-## p :: typ_all S T ->
+    G |-## p : typ_all S T ->
     G |-# S' <: S ->
     (forall y, y \notin L ->
       G & y ~ S' |- T ||^ y <: T' ||^ y) ->
-    G |-## p :: typ_all S' T'
+    G |-## p : typ_all S' T'
   (* And *)
 | t_pt_and : forall G p S T,
-    G |-## p :: S ->
-    G |-## p :: T ->
-    G |-## p :: typ_and S T
+    G |-## p : S ->
+    G |-## p : T ->
+    G |-## p : typ_and S T
   (* Tight Selection *)
 | t_pt_sel : forall G p q A S,
-    G |-## p :: S ->
-    G |-! trm_path q :: typ_rcd (dec_typ A S S) ->
+    G |-## p : S ->
+    G |-! trm_path q : typ_rcd (dec_typ A S S) ->
     norm_t G q ->
-    G |-## p :: typ_path q A
+    G |-## p : typ_path q A
   (* Top *)
 | t_pt_top : forall G p T,
-    G |-## p :: T ->
-    G |-## p :: typ_top
-where "G '|-##' p '::' T" := (tight_pt G p T).
+    G |-## p : T ->
+    G |-## p : typ_top
+where "G '|-##' p ':' T" := (tight_pt G p T).
 
 Hint Constructors tight_pt.
 
+(* ****************************************** *)
+(* Invertable to precise *)
+
+Lemma tpt_to_precise_typ_dec: forall G p A S U,
+    inert G ->
+    norm_t G p ->
+    G |-## p : typ_rcd (dec_typ A S U) ->
+    exists T,
+      G |-! trm_path p : typ_rcd (dec_typ A T T) /\
+      G |-# T <: U /\
+      G |-# S <: T.
+Proof.
+  introv HG Hn Ht.
+  dependent induction Ht.
+  - lets Hp: (precise_dec_typ_inv HG H). subst.
+    exists U. split*.
+  - specialize (IHHt A T U0 HG Hn eq_refl). destruct IHHt as [V [Hx [Hs1 Hs2]]].
+    exists V. split*.
+Qed.
+
+Lemma tpt_to_precise_trm_dec: forall G p a m T,
+    inert G ->
+    norm_t G p ->
+    G |-## p : typ_rcd {{ a [m] T }} ->
+    exists T',
+      G |-! trm_path p : typ_rcd {{ a [m] T' }} /\
+      G |-# T' <: T.
+Proof.
+  introv Hi Hn Ht. dependent induction Ht.
+  - (* t_pt_precise *)
+    exists T. auto.
+  - (* t_pt_dec_trm *)
+    specialize (IHHt _ _ _ Hi Hn eq_refl). destruct IHHt as [V [Hx Hs]].
+    exists V. split; auto.
+    eapply subtyp_trans_t; eassumption.
+Qed.
+
+Lemma tpt_to_precise_typ_all: forall G p S T,
+    inert G ->
+    norm_t G p ->
+    G |-## p : typ_all S T ->
+    exists S' T' L,
+      G |-! trm_path p : typ_all S' T' /\
+      G |-# S <: S' /\
+      (forall y,
+          y \notin L ->
+              G & y ~ S |- T' ||^ y <: T ||^ y).
+Proof.
+  introv Hi Hn Ht. dependent induction Ht.
+  - exists S T (dom G); auto.
+  - specialize (IHHt _ _ Hi Hn eq_refl).
+    destruct IHHt as [S' [T' [L' [Hpt [HSsub HTsub]]]]].
+    exists S' T' (dom G \u L \u L').
+    split; auto.
+    assert (Hsub2 : G |-# typ_all S0 T0 <: typ_all S T) by (apply* subtyp_all_t). split.
+    + eapply subtyp_trans_t; eauto.
+    + intros y Fr.
+      assert (Hok: ok (G & y ~ S)) by auto using ok_push, inert_ok.
+      apply tight_to_general in H; auto.
+      assert (Hnarrow: G & y ~ S |- T' ||^ y <: T0 ||^ y).
+      { eapply narrow_subtyping; auto using subenv_last. }
+      eauto.
+Qed.
+
+Lemma invertable_to_tight: forall G p T,
+     G |-## p : T ->
+     G |-# trm_path p : T.
+Proof.
+  introv Hi. induction Hi; eauto. apply* precise_to_tight.
+Qed.
+
 Lemma tight_possible_types_closure_tight: forall G p T U,
   inert G ->
-  G |-## p :: T ->
+  G |-## p : T ->
   G |-# T <: U ->
-  G |-## p :: U.
+  G |-## p : U.
 Proof.
   introv Hi HT Hsub.
   dependent induction Hsub; eauto.
@@ -92,17 +164,23 @@ Proof.
     + pose proof (inert_unique_tight_bounds Hi H H6). subst. assumption.
 Qed.
 
-Lemma term_path_norm_false : forall G x a T,
-    G |-## p_var (avar_f x) :: typ_rcd {{a [gen] T}} ->
-    norm_t G (p_sel (p_var (avar_f x)) a) ->
+Lemma term_path_norm_false: forall G x a T,
+    inert G ->
+    G |-## p_var (avar_f x) : typ_rcd {{a [gen] T}} ->
+    norm_p G (p_sel (p_var (avar_f x)) a) ->
     False.
-Proof. Admitted.
+Proof.
+  introv Hi Ht Hn. inversions Hn.
+  assert (norm_t G (p_var (avar_f x))) as Hx by admit.
+  destruct (tpt_to_precise_trm_dec Hi Hx Ht) as [V [Hp Hs]].
+  destruct (p_rcd_unique Hi Hp H1) as [He1 _]. inversion He1.
+Qed.
 
 Lemma tight_possible_types_lemma : forall G U p,
     inert G ->
-    G |-# trm_path p :: U ->
+    G |-# trm_path p : U ->
     norm_t G p ->
-    G |-## p :: U.
+    G |-## p : U.
 Proof.
   introv Hi Hty Hn.
   dependent induction Hty; auto.
@@ -112,12 +190,10 @@ Proof.
       destruct (typing_implies_bound Hty) as [U Hb]. apply* norm_var_t.
     }
     inversions Hn.
-    specialize (IHHty (p_var (avar_f x )) Hi eq_refl Hnx).
-
+    specialize (IHHty (p_var (avar_f x )) Hi eq_refl H4).
 
   - specialize (IHHty p0  Hi eq_refl). inversions IHHty.
     * apply ty_fld_elim_p in H. auto.
-
     specialize (IHHty _ Hgd eq_refl eq_refl eq_refl).
     eapply t_pt_bnd.
     apply IHHty.
@@ -126,4 +202,4 @@ Proof.
     inversion IHHty; subst; auto.
   - apply t_pt_and; auto.
   - eapply tight_possible_types_closure_tight; auto.
-Qed.
+Qed.*)
